library/init/meta/tactic.lean
@@ -495,7 +495,7 @@ meta constant mk_app (fn : name) (args : list expr) (md := semireducible) : tact
    ```
    returns the application
    ```
-   @ite.{1} (a > b) (nat.decidable_gt a b) nat a b
+   @ite.{1} nat (a > b) (nat.decidable_gt a b) a b
    ```
 -/
 meta constant mk_mapp (fn : name) (args : list (option expr)) (md := semireducible) : tactic expr
@@ -1570,7 +1570,7 @@ expr.sort tgt_u ← infer_type tgt >>= whnf,
 g1 ← mk_meta_var (e.imp tgt),
 g2 ← mk_meta_var (`(¬ %%e).imp tgt),
 focus1 $ do
-  exact $ expr.const ``dite [tgt_u] e inst tgt g1 g2,
+  exact $ expr.const ``dite [tgt_u] tgt e inst g1 g2,
   set_goals [g1, g2],
   all_goals' $ intro h >> skip
 
